Finished proofs for insertion sort

code/quickchick.v
@@ -47,3 +47,80 @@ Instance showTree {A} `{_ : Show A} : Show (Tree A) :=
          end
        in aux
   |}.
+
+Fixpoint genTreeSized {A} (sz : nat) (g : G A) : G (Tree A) :=
+  match sz with
+    | O => returnGen Leaf
+    | S sz' => oneOf [ returnGen Leaf ;
+                       liftGen3  Node g (genTreeSized sz' g) (genTreeSized sz' g)
+                     ]
+  end.
+
+Sample (genTreeSized 3 (choose(0,3))).
+
+Fixpoint genTreeSized' {A} (sz : nat) (g : G A) : G (Tree A) :=
+  match sz with
+    | O => returnGen Leaf 
+    | S sz' => freq [ (1,  returnGen Leaf) ;
+                       (sz, liftGen3  Node g (genTreeSized' sz' g)
+                                      (genTreeSized' sz' g))
+                    ]
+  end.
+
+Sample (genTreeSized' 3 (choose(0,3))).
+
+Fixpoint mirror {A : Type} (t : Tree A) : Tree A :=
+  match t with
+    | Leaf => Leaf
+    | Node x l r => Node x (mirror r) (mirror l)
+  end.
+
+Fixpoint eq_tree (t1 t2 : Tree nat) : bool :=
+  match t1, t2 with
+    | Leaf, Leaf => true
+    | Node x1 l1 r1, Node x2 l2 r2 =>
+      beq_nat x1 x2 && eq_tree l1 l2 && eq_tree r1 r2
+    | _, _ => false
+  end.
+
+Definition mirrorP (t : Tree nat) := eq_tree (mirror (mirror t)) t.
+
+QuickChick (forAll (genTreeSized' 5 (choose (0,5))) mirrorP).
+
+Definition faultyMirrorP (t : Tree nat) := eq_tree (mirror t) t.
+
+QuickChick (forAll (genTreeSized' 5 (choose (0,5))) faultyMirrorP).
+
+
+Open Scope list.
+
+Fixpoint shrinkTree {A} (s : A -> list A) (t : Tree A) : seq.seq (Tree A) :=
+  match t with
+    | Leaf => []
+    | Node x l r => [l] ++ [r] ++
+                    map (fun x' => Node x' l r) (s x) ++
+                    map (fun l' => Node x l' r) (shrinkTree s l) ++
+                    map (fun r' => Node x l r') (shrinkTree s r)
+  end.
+
+QuickChick (forAllShrink
+              (genTreeSized' 5 (choose (0,5))) (shrinkTree shrink) faultyMirrorP).
+
+
+Instance genTree {A} `{Gen A} : GenSized (Tree A) := 
+  {| arbitrarySized n := genTreeSized n arbitrary |}.
+
+Instance shrTree {A} `{Shrink A} : Shrink (Tree A) := 
+  {| shrink x := shrinkTree shrink x |}.
+
+QuickChick faultyMirrorP.
+
+Derive Arbitrary for Tree.
+(* genSTree is defined *)
+(* shrTree0 is defined *)
+Print genSTree.
+Print shrTree0.
+
+Derive Show for Tree.
+(* showTree0 is defined *)
+Print showTree0.
