code/insertsort.v
@@ -1,0 +1,171 @@
+From QuickChick Require Import QuickChick.
+Import QcDefaultNotation. Open Scope qc_scope.
+Import GenLow GenHigh.
+Set Warnings "-extraction-opaque-accessed,-extraction".
+Set Warnings "-notation-overridden,-parsing".
+
+Require Import mathcomp.ssreflect.ssreflect.
+From mathcomp Require Import seq ssreflect ssrbool ssrnat eqtype.
+
+Require Import List Arith_base PeanoNat String.
+Import ListNotations.
+
+Open Scope coq_nat.
+
+Section ISORT.
+
+  Fixpoint insert (x : nat)(xs : list nat) : list nat :=
+    match xs with
+    | [] => [ x ]
+    | (y :: ys) =>
+      if leb x y then x :: y :: ys else y :: (insert x ys)
+    end.
+
+  Fixpoint isort (xs : list nat) : list nat :=
+    match xs with
+    | [] => []
+    | (x :: xs) => insert x (isort xs)          
+    end.
+End ISORT.
+
+Section TEST_SPEC.
+
+  Fixpoint is_sorted (xs : list nat) : bool :=
+    match xs with
+    | [] => true
+    | [ x ] => true
+    | (x :: x' :: xs) => leb x x' && is_sorted xs
+    end.
+
+  Fixpoint elem (x : nat)(xs : list nat) : bool :=
+    match xs with
+    | [] => false
+    | (y :: ys) => beq_nat x y || elem x ys
+    end.
+  
+  Definition is_permutation (xs ys : list nat) :=
+    forallb (fun x => elem x ys) xs &&
+            forallb (fun y => elem y xs) ys.  
+  
+  Definition isort_is_sorted (xs : list nat) := is_sorted (isort xs).
+  
+  Definition isort_permutation (xs : list nat) := is_permutation xs (isort xs).
+
+  Definition isort_correct (xs : list nat) :=
+    isort_is_sorted xs && isort_permutation xs.
+
+End TEST_SPEC.
+
+QuickChick isort_correct.
+
+Section PROOF.
+
+  Inductive sorted : list nat -> Prop :=
+  | SortedNil : sorted []
+  | SortedSing : forall x, sorted [ x ]
+  | SortedRec : forall x y l, x <= y -> sorted (y :: l) -> sorted (x :: y :: l).
+
+  Hint Constructors sorted.
+
+  Require Import Omega.
+
+  Ltac inv H := inversion H ; clear H ; subst.
+
+  Lemma sorted_inv : forall x l, sorted (x :: l) -> sorted l.
+  Proof.
+    intros x l H ; inv H ; auto.
+  Qed.
+
+  Lemma insert_sorted
+    : forall l x, sorted l -> sorted (insert x l).
+  Proof.
+    intros l x H ; elim H ; simpl ; eauto.
+    intros z ; destruct (x <=? z) eqn : Heqn; simpl ; eauto.
+    +
+      apply leb_iff in Heqn ; eauto.
+    +
+      apply leb_iff_conv in Heqn.
+      assert (z <= x) by omega.
+      eauto.
+    +
+      intros.
+      destruct (x <=? y) eqn : Heqn ; destruct (x <=? x0) eqn : Heqm.
+      apply leb_iff in Heqn.
+      apply leb_iff in Heqm.
+      eauto.
+      apply leb_iff in Heqn.
+      apply leb_iff_conv in Heqm.
+      assert (x0 <= x) by omega.
+      eauto.
+      apply leb_iff_conv in Heqn.
+      apply leb_iff in Heqm.
+      eauto.
+      apply leb_iff_conv in Heqn.
+      apply leb_iff_conv in Heqm.
+      eauto.
+  Qed.
+
+  Inductive permutation {A : Type}: list A -> list A -> Prop :=
+    perm_nil : permutation [] []
+  | perm_skip : forall (x : A) (l l' : list A),
+                permutation l l' -> 
+                permutation (x :: l) (x :: l')
+  | perm_swap : forall (x y : A) (l : list A),
+                permutation (y :: x :: l) (x :: y :: l)
+  | perm_trans : forall l l' l'' : list A,
+                 permutation l l' -> 
+                 permutation l' l'' -> 
+                 permutation l l''. 
+
+  Hint Constructors permutation.
+
+  Lemma permutation_refl {A : Type}: forall (l : list A), permutation l l.
+  Proof.
+    induction l ; eauto.
+  Qed.
+
+  Lemma permutation_sym {A : Type}
+    : forall (l l' : list A), permutation l l' -> permutation l' l.
+  Proof.
+    induction 1 ; eauto.
+  Qed.
+
+  Lemma permutation_trans {A : Type}
+    : forall (l1 l2 l3 : list A), permutation l1 l2 ->
+                  permutation l2 l3 ->
+                  permutation l1 l3.
+  Proof.
+    induction 1 ; intros ; eauto.
+  Qed.
+
+  Lemma permutation_nil {A : Type} : forall (l : list A), permutation [] l -> l = [].
+  Proof.
+      intros l HF.
+      remember (@nil A) as m in HF.
+      induction HF; discriminate || auto.
+  Qed.
+
+  Lemma insert_permutation
+    : forall l x, permutation (x :: l) (insert x l).
+  Proof.
+    induction l ; intros ; simpl in * ; eauto.
+    destruct (x <=? a) eqn : Ha ; eauto.
+  Qed.
+
+  Lemma isort_permutation_thm : forall l, permutation l (isort l).
+  Proof.
+    Hint Resolve insert_permutation.
+    induction l ; simpl in * ; eauto.
+  Qed.
+
+  Theorem isort_correct_thm : forall l, permutation l (isort l) /\
+                                   sorted (isort l).
+  Proof.
+    induction l ; split ; simpl ; eauto.
+    +
+      destruct IHl ; simpl ; eauto.
+    +
+      destruct IHl.
+      apply insert_sorted ; auto.
+  Qed.
+End PROOF. 
